new atom_cond def; update lower_atom_cond

src/phase2/freedom_of_action.lean
@@ -497,16 +497,22 @@ lemma graph_struct_perm (σ : spec B) (hσ₁ : σ.one_to_one_forward B) (hσ₂
 
 /-- The allowability condition on atoms.
 In an absent litter, we must specify only `< κ`-many atoms.
-In a present litter, we can specify either `< κ`-many atoms, or all of the atoms in the litter, and
-in this case, almost all of them must be mapped to the right place.
+In a present litter, we can specify either `< κ`-many atoms and they are mapped to the right place,
+or all of the atoms in the litter, and their range is exactly the image of the litter.
 Note that the `small` constructor does not depend on whether the litter is present or absent. -/
 @[mk_iff] inductive atom_cond (σ : spec B) (L : litter) (A : extended_index B) : Prop
-| small : small {a ∈ litter_set L | (⟨sum.inl a, A⟩ : support_condition B) ∈ σ.domain} → atom_cond
-| all (N : near_litter) (atom_map : litter_set L → atom) :
-    (⟨sum.inr ⟨L.to_near_litter, N⟩, A⟩ : binary_condition B) ∈ σ →
-    (∀ a ∈ litter_set L, (⟨sum.inl ⟨a, atom_map ⟨a, ‹_›⟩⟩, A⟩ : binary_condition B) ∈ σ) →
-    N.snd.val = set.range atom_map →
-    atom_cond
+| all
+    (N : near_litter) (hL : (⟨sum.inr ⟨L.to_near_litter, N⟩, A⟩ : binary_condition B) ∈ σ)
+    (atom_map : litter_set L → atom) :
+  (∀ a ∈ litter_set L, (⟨sum.inl ⟨a, atom_map ⟨a, ‹_›⟩⟩, A⟩ : binary_condition B) ∈ σ) →
+  N.snd.val = set.range atom_map → atom_cond
+| small_out
+    (hL : (sum.inr L.to_near_litter, A) ∉ σ.domain) :
+  small {a ∈ litter_set L | (⟨sum.inl a, A⟩ : support_condition B) ∈ σ.domain} → atom_cond
+| small_in
+    (N : near_litter) (hL : (sum.inr (L.to_near_litter, N), A) ∈ σ) :
+  small {a ∈ litter_set L | (⟨sum.inl a, A⟩ : support_condition B) ∈ σ.domain} →
+  (∀ (a ∈ litter_set L) (b : atom), (sum.inl (a, b), A) ∈ σ → b ∈ N.snd.val) → atom_cond
 
 /-- The allowability condition on near-litters.
 If a near-litter is present, so are its litter and all atoms in the symmetric difference, and it is
@@ -622,18 +628,24 @@ lemma lower_atom_cond (hσ : σ.allowable_spec B) :
 begin
   intros L C,
   unfold spec.lower binary_condition.extend_path,
-  obtain hsmall | ⟨N, atom_map, h1, h2, h3⟩ := hσ.forward.atom_cond L (A.comp C),
-  { refine spec.atom_cond.small _,
-    convert hsmall,
+  obtain ⟨hL, hsmall⟩ | ⟨N, hL, hsmall, hmaps⟩ | ⟨N, atom_map, h1, h2, h3⟩ := hσ.forward.atom_cond L (A.comp C),
+  { exact spec.atom_cond.all N atom_map h1 h2 h3 },
+  { refine spec.atom_cond.small_out _ _,
+    { convert hL using 1,
+      refine eq_iff_iff.2 ⟨_, _⟩; rintro ⟨⟨_ | ⟨x, y⟩, C⟩, hbin, hdom⟩; cases hdom,
+      { exact ⟨_, hbin, prod.mk.inj_iff.2 ⟨(prod.mk.inj hdom).1, rfl⟩⟩ },
+      { exact ⟨(sum.inr (L.to_near_litter, y), C), hbin, prod.mk.inj_iff.2 ⟨(prod.mk.inj hdom).1, rfl⟩⟩ } } },
+  swap,
+  { refine spec.atom_cond.small_in N hL _ hmaps },
+  all_goals { convert hsmall,
     unfold spec.domain binary_condition.domain,
     ext a,
-    simp,
+    simp only [set.mem_image, prod.mk.inj_iff],
     split; rintro ⟨⟨x, y⟩, hx1, hx2, hx3⟩,
     { exact ⟨⟨x, A.comp y⟩, hx1, hx2, by rw ← hx3⟩ },
     dsimp only at hx3,
     rw hx3 at hx1 hx2,
-    exact ⟨⟨x, C⟩, hx1, hx2, rfl⟩ },
-  { exact spec.atom_cond.all N atom_map h1 h2 h3 }
+    exact ⟨⟨x, C⟩, hx1, hx2, rfl⟩ }
 end
 
 lemma lower_near_litter_cond (hσ : σ.allowable_spec B) :
